preservation: proven, yay!!

Capless/Weakening/Basic.lean
@@ -17,6 +17,14 @@ def VarMap.weaken_ext {Γ : Context n m k} :
   apply VarMap.ext
   apply VarMap.weaken
 
+def VarMap.lweaken_ext {Γ : Context n m k} :
+  VarMap
+    (Γ.var T)
+    FinFun.weaken.ext
+    ((Γ.label P).var T.weaken) := by
+  apply VarMap.ext
+  apply VarMap.lweaken
+
 def VarMap.weaken_cext_ext {Γ : Context n m k} :
   VarMap
     ((Γ.cvar CBinding.bound).var T)
@@ -25,6 +33,15 @@ def VarMap.weaken_cext_ext {Γ : Context n m k} :
   apply VarMap.ext
   apply VarMap.cext
   apply VarMap.weaken
+
+def VarMap.lweaken_cext_ext {Γ : Context n m k} :
+  VarMap
+    ((Γ.cvar CBinding.bound).var T)
+    FinFun.weaken.ext
+    (((Γ.label P).cvar CBinding.bound).var T.weaken) := by
+  apply VarMap.ext
+  apply VarMap.cext
+  apply VarMap.lweaken
 
 def CVarMap.weaken {Γ : Context n m k} :
   CVarMap Γ FinFun.weaken (Γ.cvar b) := by
