Capless/Weakening/TypedCont.lean
@@ -1,4 +1,3 @@
 import Capless.Weakening.TypedCont.Term
 import Capless.Weakening.TypedCont.Type
 import Capless.Weakening.TypedCont.Capture
-import Capless.Weakening.TypedCont.Label
