Capless/Weakening/TypedCont/Term.lean
@@ -113,4 +113,91 @@ theorem TypedCont.weaken
     { aesop }
     { apply hs.weaken }
 
+theorem Cont.HasLabel.lweaken
+  (h : Cont.HasLabel cont x tail) :
+  Cont.HasLabel cont.weaken x.succ tail.weaken := by
+  induction h
+  case here =>
+    simp [Cont.weaken]
+    apply here
+  case there_val ih =>
+    simp [Cont.weaken]
+    apply there_val; trivial
+  case there_tval ih =>
+    simp [Cont.weaken]
+    apply there_tval; trivial
+  case there_cval ih =>
+    simp [Cont.weaken]
+    apply there_cval; trivial
+  case there_label ih =>
+    simp [Cont.weaken]
+    apply there_label; trivial
+
+theorem WellScoped.lweaken
+  (h : WellScoped Γ cont Ct) :
+  WellScoped (Γ.label S) cont.weaken Ct.weaken := by
+  induction h
+  case empty => simp [CaptureSet.weaken]; constructor
+  case union ih1 ih2 =>
+    simp [CaptureSet.weaken] at *
+    apply union <;> aesop
+  case singleton hb _ ih =>
+    apply singleton
+    { simp [FinFun.weaken]
+      have hb1 := Context.Bound.there_label (S:=S) hb
+      simp [CaptureSet.weaken, CaptureSet.rename] at hb1
+      exact hb1 }
+    { exact ih }
+  case csingleton hb _ ih =>
+    apply csingleton
+    { have hb1 := Context.CBound.there_label (S:=S) hb
+      exact hb1 }
+    { exact ih }
+  case label hb hs =>
+    apply label
+    { have hb1 := Context.LBound.there_label (S':=S) hb
+      exact hb1 }
+    { apply hs.lweaken }
+
+theorem TypedCont.lweaken
+  (h : TypedCont Γ E cont E' Ct) :
+  TypedCont (Γ.label S) E.weaken cont.weaken E'.weaken Ct.weaken := by
+  induction h
+  case none =>
+    simp [Cont.weaken]
+    apply none
+    apply? ESubtyp.lweaken
+  case cons ih =>
+    simp [Cont.weaken]
+    have heq : ∀ {n m k} {T0 : CType n m k}, (EType.type T0).weaken = EType.type T0.weaken := by
+      intro T0
+      simp [EType.weaken, EType.rename, CType.weaken]
+    rw [heq]
+    apply cons
+    { rename_i ht _ _
+      have ht1 := ht.lweaken_ext (P := S)
+      rw [EType.weaken1_weaken] at ht1
+      rw [CaptureSet.weaken1_weaken] at ht1
+      exact ht1 }
+    { apply WellScoped.lweaken; assumption }
+    { exact ih }
+  case conse ih =>
+    simp [Cont.weaken, EType.weaken_ex]
+    apply conse
+    { rename_i ht _ _
+      have ht1 := ht.lweaken_cext_ext (P := S)
+      rw [EType.weaken1_weaken] at ht1
+      rw [EType.weaken_cweaken] at ht1
+      rw [CaptureSet.weaken1_weaken] at ht1
+      rw [CaptureSet.weaken_cweaken] at ht1
+      exact ht1 }
+    { apply WellScoped.lweaken; aesop }
+    { exact ih }
+  case scope hs ih =>
+    simp [Cont.weaken]
+    apply scope
+    { constructor; aesop }
+    { aesop }
+    { apply hs.lweaken }
+
 end Capless
